restructatization

code/experimental/P256/Hacl.Impl.LowLevel.fst
@@ -35,7 +35,6 @@ let add_carry cin x y result1 =
   c
 
 
-inline_for_extraction noextract
 val add4: x: felem -> y: felem -> result: felem -> 
   Stack uint64
     (requires fun h -> live h x /\ live h y /\ live h result /\ eq_or_disjoint x result /\ eq_or_disjoint y result)
@@ -62,7 +61,6 @@ let add4 x y result =
     cc
 
 
-inline_for_extraction noextract
 val add4_variables: x: felem -> cin: uint64 {uint_v cin <=1} ->  y0: uint64 -> y1: uint64 -> y2: uint64 -> y3: uint64 -> result: felem -> 
   Stack uint64
     (requires fun h -> live h x /\ live h result /\ eq_or_disjoint x result)
@@ -94,13 +92,7 @@ let add4_variables x cin y0 y1 y2 y3 result =
 val sub_borrow: cin: uint64{uint_v cin <= 1} -> x: uint64 -> y: uint64 -> r: lbuffer uint64 (size 1) -> 
   Stack uint64
     (requires fun h -> live h r)
-    (ensures fun h0 c h1 -> modifies1 r h0 h1 /\ 
-      (
-  let r = as_seq h1 r in 
-  let r = Seq.index r 0 in 
-  v r - v c * pow2 64 == v x - v y - v cin)
-      )
-
+    (ensures fun h0 c h1 -> modifies1 r h0 h1 /\ (let r = Seq.index (as_seq h1 r) 0 in v r - v c * pow2 64 == v x - v y - v cin))
 
 let sub_borrow cin x y result1 = 
   let res = x -. y -. cin in
@@ -118,11 +110,9 @@ val sub4_il: x: felem -> y: ilbuffer uint64 (size 4) -> result: felem ->
     (requires fun h -> live h x /\ live h y /\ live h result /\ disjoint x result /\ disjoint y result)
     (ensures fun h0 c h1 -> modifies1 result h0 h1 /\ v c <= 1 /\
       (
-  let result = as_seq h1 result in 
-  let x = as_seq h0 x in 
-  let y = as_seq h0 y in 
-  felem_seq_as_nat result - v c * pow2 256 == felem_seq_as_nat x - felem_seq_as_nat y /\
-  (if uint_v c = 0 then felem_seq_as_nat x >= felem_seq_as_nat y else felem_seq_as_nat x < felem_seq_as_nat y)
+	let y = as_seq h0 y in 
+ 	as_nat h1 result - v c * pow2 256 == as_nat h0 x  - felem_seq_as_nat y /\
+	(if uint_v c = 0 then as_nat h0 x >= felem_seq_as_nat y else as_nat h0 x < felem_seq_as_nat y)
       )
    )
 
@@ -142,31 +132,25 @@ let sub4_il x y result =
 val sub4: x: felem -> y:felem -> result: felem -> 
   Stack uint64
     (requires fun h -> live h x /\ live h y /\ live h result /\ eq_or_disjoint x result /\ eq_or_disjoint y result)
-    (ensures fun h0 c h1 -> modifies1 result h0 h1 /\ v c <= 1 /\
-      (
-  let result = as_seq h1 result in 
-  let x = as_seq h0 x in 
-  let y = as_seq h0 y in 
-  felem_seq_as_nat result - v c * pow2 256 == felem_seq_as_nat x - felem_seq_as_nat y
-      )
-   )
+    (ensures fun h0 c h1 -> modifies1 result h0 h1 /\ v c <= 1 /\ as_nat h1 result - v c * pow2 256 == as_nat h0 x - as_nat h0 y)
 
 let sub4 x y result = 
-    let r0 = sub result (size 0) (size 1) in 
-    let r1 = sub result (size 1) (size 1) in 
-    let r2 = sub result (size 2) (size 1) in 
-    let r3 = sub result (size 3) (size 1) in 
+  let h0 = ST.get() in 
+	
+  let r0 = sub result (size 0) (size 1) in 
+  let r1 = sub result (size 1) (size 1) in 
+  let r2 = sub result (size 2) (size 1) in 
+  let r3 = sub result (size 3) (size 1) in 
       
-      let h0 = ST.get() in 
-    let cc = sub_borrow (u64 0) x.(size 0) y.(size 0) r0 in 
-    let cc = sub_borrow cc x.(size 1) y.(size 1) r1 in 
-    let cc = sub_borrow cc x.(size 2) y.(size 2) r2 in 
-    let cc = sub_borrow cc x.(size 3) y.(size 3) r3 in 
+  let cc = sub_borrow (u64 0) x.(size 0) y.(size 0) r0 in 
+  let cc = sub_borrow cc x.(size 1) y.(size 1) r1 in 
+  let cc = sub_borrow cc x.(size 2) y.(size 2) r2 in 
+  let cc = sub_borrow cc x.(size 3) y.(size 3) r3 in 
     
     assert(let r1_0 = as_seq h0 r1 in let r0_ = as_seq h0 result in Seq.index r0_ 1 == Seq.index r1_0 0);
     assert(let r2_0 = as_seq h0 r2 in let r0_ = as_seq h0 result in Seq.index r0_ 2 == Seq.index r2_0 0);
     assert(let r3_0 = as_seq h0 r3 in let r0_ = as_seq h0 result in Seq.index r0_ 3 == Seq.index r3_0 0);
-    cc
+  cc
 
 
 
@@ -174,13 +158,7 @@ val cmovznz4: cin: uint64 -> x: felem -> y: felem -> result: felem ->
   Stack unit
     (requires fun h -> live h x /\ live h y /\ live h result /\ disjoint x result /\ eq_or_disjoint y result)
     (ensures fun h0 _ h1 -> modifies1 result h0 h1 /\ 
-      (
-  let r = as_seq h1 result in 
-  let x = as_seq h0 x in 
-  let y = as_seq h0 y in 
-  if uint_v cin = 0 then felem_seq_as_nat r == felem_seq_as_nat x else felem_seq_as_nat r == felem_seq_as_nat y
-      )
-    )
+      (if uint_v cin = 0 then as_nat h1 result == as_nat h0 x else as_nat h1 result == as_nat h0 y))
 
 let cmovznz4 cin x y r =  
   let h0 = ST.get() in 
@@ -195,8 +173,8 @@ let cmovznz4 cin x y r =
   upd r (size 2) r2;
   upd r (size 3) r3;
 
-  let x = as_seq h0 x in 
-  let y = as_seq h0 y in 
+    let x = as_seq h0 x in 
+    let y = as_seq h0 y in 
     
     cmovznz4_lemma cin (Seq.index x 0) (Seq.index y 0);
     cmovznz4_lemma cin (Seq.index x 1) (Seq.index y 1);
@@ -204,7 +182,32 @@ let cmovznz4 cin x y r =
     cmovznz4_lemma cin (Seq.index x 3) (Seq.index y 3)
 
 
-#reset-options "--z3refresh --z3rlimit 200"
+val shift_256_impl: i: felem -> o: lbuffer uint64 (size 8) -> 
+  Stack unit 
+    (requires fun h -> live h i /\ live h o /\ disjoint i o)
+    (ensures fun h0 _ h1 -> modifies1 o h0 h1 /\ 
+      (
+	let o = as_seq h1 o in 
+	felem_seq_as_nat_8 o == as_nat h0 i * pow2 256 
+      )
+    )
+
+let shift_256_impl i o = 
+  upd o (size 0) (u64 0);
+  upd o (size 1) (u64 0);
+  upd o (size 2) (u64 0);
+  upd o (size 3) (u64 0);
+  upd o (size 4) i.(size 0);
+  upd o (size 5) i.(size 1);
+  upd o (size 6) i.(size 2);
+  upd o (size 7) i.(size 3);
+
+  assert_norm(pow2 64 * pow2 64 * pow2 64 = pow2 192);
+  assert_norm(pow2 64 * pow2 64 * pow2 64 * pow2 64 = pow2 256);
+  assert_norm(pow2 64 * pow2 64 * pow2 64  * pow2 64 * pow2 64= pow2 (5 * 64));
+  assert_norm(pow2 64 * pow2 64 * pow2 64  * pow2 64 * pow2 64 * pow2 64 = pow2 (6 * 64));
+  assert_norm(pow2 64 * pow2 64 * pow2 64  * pow2 64 * pow2 64* pow2 64 * pow2 64 = pow2 (7 * 64));
+  assert_norm(pow2 64 * pow2 64 * pow2 64  * pow2 64 * pow2 64* pow2 64 * pow2 64 * pow2 64 = pow2 (8 * 64))
 
 
 inline_for_extraction
@@ -250,90 +253,3 @@ let reduction_prime_2prime_impl x result =
   pop_frame()  
 
 
-inline_for_extraction noextract
-val reduction_prime256_2prime256_with_carry_impl: cin: uint64 -> x: felem -> result: felem ->
-  Stack unit 
-    (requires fun h -> live h x /\ live h result /\  eq_or_disjoint x result /\ 
-      (let x = as_seq h x in  felem_seq_as_nat x + uint_v cin * pow2 256) < 2 * prime256)
-    (ensures fun h0 _ h1 -> modifies1 result h0 h1 /\ 
-      (
-  let r = as_seq h1 result in 
-  let x = as_seq h0 x in 
-  felem_seq_as_nat r = (felem_seq_as_nat x + uint_v cin * pow2 256) % prime256
-      )
-    )  
-
-
-let reduction_prime256_2prime256_with_carry_impl cin x result = 
-  push_frame();
-    let tempBuffer = create (size 4) (u64 0) in 
-    let tempBufferForSubborrow = create (size 1) (u64 0) in 
-    recall_contents prime256_buffer (Lib.Sequence.of_list p256_prime_list);
-      let h0  = ST.get() in 
-    let c = sub4_il x prime256_buffer tempBuffer in
-      let h1 = ST.get() in 
-	assert(let x = felem_seq_as_nat (as_seq h0 x) in if x < prime256 then uint_v c = 1 else uint_v c = 0);
-	assert(felem_seq_as_nat (as_seq h1 tempBuffer)  = felem_seq_as_nat (as_seq h0 x) - prime256 + uint_v c * pow2 256);
-    let carry = sub_borrow c cin (u64 0) tempBufferForSubborrow in 
-      assert(if uint_v cin > 0 then uint_v carry == 0 else if uint_v c = 0 then uint_v carry = 0 else uint_v carry = 1);
-      cmovznz4 carry tempBuffer x result;
-      let h3 = ST.get() in 
-      modulo_addition_lemma (felem_seq_as_nat (as_seq h3 result)) prime256 1;
-      assert((felem_seq_as_nat (as_seq h3 result) + prime256) % prime256 = (felem_seq_as_nat (as_seq h3 result)) % prime256);
-      small_modulo_lemma_1 (as_nat h3 result) prime256;
-      assert(let resultN = felem_seq_as_nat (as_seq h3 result) in 
-	if uint_v cin = 1 then 
-	  if uint_v c = 0 then 
-	    resultN = felem_seq_as_nat (as_seq h0 x) - prime256 /\
-	    (felem_seq_as_nat (as_seq h0 x) + uint_v cin * pow2 256) % prime256 = resultN
-	  else 
-	    resultN = felem_seq_as_nat (as_seq h0 x) - prime256 + pow2 256 /\
-	    resultN < prime256 /\
-	    resultN % prime256 == resultN  /\
-	    (felem_seq_as_nat (as_seq h0 x) + uint_v cin * pow2 256) % prime256 == resultN  
-       else 
-        True );
-
-      assert(let resultN = felem_seq_as_nat (as_seq h3 result) in 
-	if uint_v cin = 0 then 
-	  if uint_v c = 0 then 
-	    uint_v carry = 0 /\
-	    resultN = felem_seq_as_nat (as_seq h0 x) - prime256 /\
-	    (felem_seq_as_nat (as_seq h0 x) + uint_v carry * pow2 256) % prime256  == resultN
-	  else 
-	    uint_v carry = 1 /\
-	    resultN = felem_seq_as_nat (as_seq h0 x) /\
-	    (felem_seq_as_nat (as_seq h0 x) + uint_v cin * pow2 256) % prime256  = resultN % prime256 
-	  else True  );
- 
- pop_frame()   
-
-
-
-val shift_256_impl: i: felem -> o: lbuffer uint64 (size 8) -> 
-  Stack unit 
-    (requires fun h -> live h i /\ live h o /\ disjoint i o)
-    (ensures fun h0 _ h1 -> modifies1 o h0 h1 /\ 
-      (
-  let i = as_seq h0 i in 
-  let o = as_seq h1 o in 
-  felem_seq_as_nat_8 o == felem_seq_as_nat i * pow2 256 
-      )
-    )
-
-let shift_256_impl i o = 
-  upd o (size 0) (u64 0);
-  upd o (size 1) (u64 0);
-  upd o (size 2) (u64 0);
-  upd o (size 3) (u64 0);
-  upd o (size 4) i.(size 0);
-  upd o (size 5) i.(size 1);
-  upd o (size 6) i.(size 2);
-  upd o (size 7) i.(size 3);
-
-  assert_norm(pow2 64 * pow2 64 * pow2 64 = pow2 192);
-  assert_norm(pow2 64 * pow2 64 * pow2 64 * pow2 64 = pow2 256);
-  assert_norm(pow2 64 * pow2 64 * pow2 64  * pow2 64 * pow2 64= pow2 (5 * 64));
-  assert_norm(pow2 64 * pow2 64 * pow2 64  * pow2 64 * pow2 64 * pow2 64 = pow2 (6 * 64));
-  assert_norm(pow2 64 * pow2 64 * pow2 64  * pow2 64 * pow2 64* pow2 64 * pow2 64 = pow2 (7 * 64));
-  assert_norm(pow2 64 * pow2 64 * pow2 64  * pow2 64 * pow2 64* pow2 64 * pow2 64 * pow2 64 = pow2 (8 * 64))
