code/experimental/P256/Hacl.Impl.P256.LowLevel.fst
@@ -20,6 +20,67 @@ open FStar.Mul
 
 #reset-options "--z3refresh --z3rlimit 100"
 
+
+inline_for_extraction noextract
+val reduction_prime256_2prime256_with_carry_impl: cin: uint64 -> x: felem -> result: felem ->
+  Stack unit 
+    (requires fun h -> live h x /\ live h result /\  eq_or_disjoint x result /\ 
+      (let x = as_seq h x in  felem_seq_as_nat x + uint_v cin * pow2 256) < 2 * prime256)
+    (ensures fun h0 _ h1 -> modifies1 result h0 h1 /\ 
+      (
+  let r = as_seq h1 result in 
+  let x = as_seq h0 x in 
+  felem_seq_as_nat r = (felem_seq_as_nat x + uint_v cin * pow2 256) % prime256
+      )
+    )  
+
+
+let reduction_prime256_2prime256_with_carry_impl cin x result = 
+  push_frame();
+    let tempBuffer = create (size 4) (u64 0) in 
+    let tempBufferForSubborrow = create (size 1) (u64 0) in 
+    recall_contents prime256_buffer (Lib.Sequence.of_list p256_prime_list);
+      let h0  = ST.get() in 
+    let c = sub4_il x prime256_buffer tempBuffer in
+      let h1 = ST.get() in 
+	assert(let x = felem_seq_as_nat (as_seq h0 x) in if x < prime256 then uint_v c = 1 else uint_v c = 0);
+	assert(felem_seq_as_nat (as_seq h1 tempBuffer)  = felem_seq_as_nat (as_seq h0 x) - prime256 + uint_v c * pow2 256);
+    let carry = sub_borrow c cin (u64 0) tempBufferForSubborrow in 
+      assert(if uint_v cin > 0 then uint_v carry == 0 else if uint_v c = 0 then uint_v carry = 0 else uint_v carry = 1);
+      cmovznz4 carry tempBuffer x result;
+      let h3 = ST.get() in 
+      modulo_addition_lemma (felem_seq_as_nat (as_seq h3 result)) prime256 1;
+      assert((felem_seq_as_nat (as_seq h3 result) + prime256) % prime256 = (felem_seq_as_nat (as_seq h3 result)) % prime256);
+      small_modulo_lemma_1 (as_nat h3 result) prime256;
+      assert(let resultN = felem_seq_as_nat (as_seq h3 result) in 
+	if uint_v cin = 1 then 
+	  if uint_v c = 0 then 
+	    resultN = felem_seq_as_nat (as_seq h0 x) - prime256 /\
+	    (felem_seq_as_nat (as_seq h0 x) + uint_v cin * pow2 256) % prime256 = resultN
+	  else 
+	    resultN = felem_seq_as_nat (as_seq h0 x) - prime256 + pow2 256 /\
+	    resultN < prime256 /\
+	    resultN % prime256 == resultN  /\
+	    (felem_seq_as_nat (as_seq h0 x) + uint_v cin * pow2 256) % prime256 == resultN  
+       else 
+        True );
+
+      assert(let resultN = felem_seq_as_nat (as_seq h3 result) in 
+	if uint_v cin = 0 then 
+	  if uint_v c = 0 then 
+	    uint_v carry = 0 /\
+	    resultN = felem_seq_as_nat (as_seq h0 x) - prime256 /\
+	    (felem_seq_as_nat (as_seq h0 x) + uint_v carry * pow2 256) % prime256  == resultN
+	  else 
+	    uint_v carry = 1 /\
+	    resultN = felem_seq_as_nat (as_seq h0 x) /\
+	    (felem_seq_as_nat (as_seq h0 x) + uint_v cin * pow2 256) % prime256  = resultN % prime256 
+	  else True  );
+ 
+ pop_frame()   
+
+
+
 val lemma_t_computation: t: uint64{uint_v t == 0 \/ uint_v t == 1} -> 
   Lemma
     (
